WIP on EveryEntryWasCreated

raft-proofs/EveryEntryWasCreatedProof.v
@@ -8,9 +8,16 @@ Require Import Net.
 Require Import Raft.
 Require Import RaftRefinementInterface.
 Require Import CommonDefinitions.
+Require Import RefinementCommonDefinitions.
 
 Require Import LeadersHaveLeaderLogsInterface.
 Require Import EveryEntryWasCreatedInterface.
+Require Import SpecLemmas.
+Require Import RefinementSpecLemmas.
+Require Import CommonTheorems.
+
+Require Import UpdateLemmas.
+Local Arguments update {_} {_} {_} _ _ _ _ : simpl never.
 
 Section EveryEntryWasCreated.
   Context {orig_base_params : BaseParams}.
@@ -29,12 +36,205 @@ Section EveryEntryWasCreated.
   | in_ll : forall h t ll, In (t, ll) (leaderLogs (fst (nwState net h))) ->
                       In e ll ->
                       in_any_log net e.
-
+  Hint Constructors in_any_log.
   (* proof sketch: prove for in_any_log. the only time new entries
   come into the system is on a leader, and leaders have leaderLogs in
   their term.  *)
 
-  Instance eewci : every_entry_was_created_interface.
+  Definition in_any_log_term_was_created net :=
+    forall e,
+      in_any_log net e ->
+      term_was_created net (eTerm e).
+
+  Ltac iae_case :=
+    match goal with
+      | [ H : in_any_log _ _ |- _ ] => invcs H
+    end.
+
+  Lemma term_was_created_preserved :
+    forall net net' t,
+      term_was_created net t ->
+      (forall h t ll,
+         In (t, ll) (leaderLogs (fst (nwState net h))) ->
+         In (t, ll) (leaderLogs (fst (nwState net' h)))) ->
+      term_was_created net' t.
+  Proof.
+    intros. unfold term_was_created in *.
+    break_exists_exists. eauto.
+  Qed.
+
+  
+  Ltac update_destruct :=
+    match goal with
+      | [ |- context [ update _ ?y _ ?x ] ] => destruct (name_eq_dec y x)
+    end.
+
+  Ltac update_destruct_hyp :=
+    match goal with
+      | [ _ : context [ update _ ?y _ ?x ] |- _ ] => destruct (name_eq_dec y x)
+    end.
+
+  Ltac destruct_update :=
+    repeat (first [update_destruct_hyp|update_destruct]; subst; rewrite_update).
+
+  Ltac in_aer :=
+    repeat find_rewrite; eapply in_aer; eauto; repeat find_rewrite; reflexivity.
+
+  Lemma in_any_log_term_was_created_append_entries :
+    refined_raft_net_invariant_append_entries in_any_log_term_was_created.
+  Proof.
+    red. intros. unfold in_any_log_term_was_created. intros.
+    eapply term_was_created_preserved; [eapply_prop in_any_log_term_was_created|];
+    [|
+     intros; simpl in *;
+     repeat find_higher_order_rewrite;
+     destruct_update; simpl in *; eauto;
+     rewrite update_elections_data_appendEntries_leaderLogs; eauto].
+    iae_case.
+    - repeat find_higher_order_rewrite.
+      destruct_update; simpl in *; eauto.
+      find_apply_lem_hyp handleAppendEntries_log. intuition; try in_aer.
+      + repeat find_rewrite. eauto.
+      + repeat find_rewrite. do_in_app. intuition; try in_aer.
+        eauto using removeAfterIndex_in.
+    - find_eapply_lem_hyp handleAppendEntries_not_append_entries.
+      find_apply_hyp_hyp. intuition.
+      + match goal with
+          | _ : In ?p' (_ ++ _) |- _ => eapply in_aer with (p := p'); eauto
+        end.
+      + subst. simpl in *.
+        find_false. unfold mEntries in *.
+        break_match; try congruence. subst.
+        repeat eexists; eauto.
+    - repeat find_higher_order_rewrite.
+      destruct_update; simpl in *; eauto.
+      find_rewrite_lem update_elections_data_appendEntries_leaderLogs.
+      eauto.
+  Qed.
+
+  Lemma in_any_log_term_was_created_request_vote :
+    refined_raft_net_invariant_request_vote in_any_log_term_was_created.
+  Proof.
+    red. intros. unfold in_any_log_term_was_created. intros.
+    eapply term_was_created_preserved; [eapply_prop in_any_log_term_was_created|];
+    [|
+     intros; simpl in *;
+     repeat find_higher_order_rewrite;
+     destruct_update; simpl in *; eauto;
+     rewrite leaderLogs_update_elections_data_requestVote; eauto].
+    iae_case.
+    - repeat find_higher_order_rewrite.
+      destruct_update; simpl in *; eauto.
+      find_apply_lem_hyp handleRequestVote_log.
+      repeat find_rewrite. eauto.
+    - find_eapply_lem_hyp handleRequestVote_no_append_entries.
+      find_apply_hyp_hyp. intuition.
+      + match goal with
+          | _ : In ?p' (_ ++ _) |- _ => eapply in_aer with (p := p'); eauto
+        end.
+      + subst. simpl in *.
+        find_false. unfold mEntries in *.
+        break_match; try congruence. subst.
+        repeat eexists; eauto.
+    - repeat find_higher_order_rewrite.
+      destruct_update; simpl in *; eauto.
+      find_rewrite_lem leaderLogs_update_elections_data_requestVote.
+      eauto.
+  Qed.
+
+  Lemma in_any_log_term_was_created_append_entries_reply :
+    refined_raft_net_invariant_append_entries_reply in_any_log_term_was_created.
+  Proof.
+    red. intros. unfold in_any_log_term_was_created. intros.
+    eapply term_was_created_preserved; [eapply_prop in_any_log_term_was_created|];
+    [|
+     intros; simpl in *;
+     repeat find_higher_order_rewrite;
+     destruct_update; simpl in *; eauto].
+    iae_case.
+    - repeat find_higher_order_rewrite.
+      destruct_update; simpl in *; eauto.
+      find_apply_lem_hyp handleAppendEntriesReply_log.
+      repeat find_rewrite. eauto.
+    - find_eapply_lem_hyp handleAppendEntriesReply_packets.
+      find_apply_hyp_hyp. intuition.
+      + match goal with
+          | _ : In ?p' (_ ++ _) |- _ => eapply in_aer with (p := p'); eauto
+        end.
+      + subst. simpl in *. intuition.
+    - repeat find_higher_order_rewrite.
+      destruct_update; simpl in *; eauto.
+  Qed.
+
+  Lemma in_any_log_term_was_created_request_vote_reply :
+    refined_raft_net_invariant_request_vote_reply in_any_log_term_was_created.
+  Proof.
+    red. intros. unfold in_any_log_term_was_created. intros.
+    eapply term_was_created_preserved; [eapply_prop in_any_log_term_was_created|];
+    [|intros; simpl in *;
+      repeat find_higher_order_rewrite;
+      destruct_update; simpl in *; eauto;
+      eapply update_elections_data_requestVoteReply_old; eauto].
+    iae_case.
+    - repeat find_higher_order_rewrite.
+      destruct_update; simpl in *; eauto.
+      find_rewrite_lem handleRequestVoteReply_log_rewrite; eauto.
+    - find_apply_hyp_hyp.
+      match goal with
+        | _ : In ?p' (_ ++ _) |- _ => eapply in_aer with (p := p'); eauto
+      end.
+    - repeat find_higher_order_rewrite.
+      destruct_update; simpl in *; eauto.
+      find_eapply_lem_hyp leaderLogs_update_elections_data_RVR; eauto.
+      intuition; eauto. subst.
+      find_rewrite_lem handleRequestVoteReply_log_rewrite. eauto.
+  Qed.
+
+  Ltac in_log_in_leader_log :=
+    find_eapply_lem_hyp in_log; eapply_prop_hyp in_any_log_term_was_created in_any_log;
+    unfold term_was_created in *;
+    break_exists_exists;
+    find_higher_order_rewrite;
+    destruct_update; simpl in *; eauto;
+    rewrite update_elections_data_client_request_leaderLogs; eauto.
+
+  Lemma in_any_log_term_was_created_client_request :
+    refined_raft_net_invariant_client_request in_any_log_term_was_created.
+  Proof.
+    red. intros. unfold in_any_log_term_was_created. intros.
+    iae_case.
+    - unfold term_was_created. simpl in *.
+      find_higher_order_rewrite.
+      destruct_update; simpl in *; eauto.
+      + find_apply_lem_hyp handleClientRequest_log.
+        intuition; subst; repeat find_rewrite; try in_log_in_leader_log.
+        break_exists. intuition.
+        repeat find_rewrite. simpl in *. intuition; subst.
+        * find_eapply_lem_hyp leaders_have_leaderLogs_invariant; eauto.
+          match goal with
+            | [h : name |- _ ] => (exists h)
+          end.
+          break_exists_exists.
+          repeat find_rewrite.
+          repeat find_higher_order_rewrite.
+          rewrite update_eq; auto. simpl.
+          rewrite update_elections_data_client_request_leaderLogs.
+          auto.
+        * in_log_in_leader_log.
+      + in_log_in_leader_log.
+    -
   Admitted.
+      
+  Theorem in_any_log_term_was_created_invariant :
+    forall net,
+      refined_raft_intermediate_reachable net ->
+      in_any_log_term_was_created net.
+  Admitted.
+
+  Instance eewci : every_entry_was_created_interface.
+  split.
+  unfold every_entry_was_created. intros.
+  apply in_any_log_term_was_created_invariant; eauto.
+  Qed.
 
 End EveryEntryWasCreated.
